Fix the EL offset issue

x86/proofs/mlkem_keccak_f1600_loop_no_stack.ml
@@ -15,6 +15,7 @@
  (**** print_literal_from_elf "x86/mlkem/mlkem_keccak_f1600_no_stack.o";;
  ****)
 
+
 let GHOST_REGLIST_TAC =
   W(fun (asl,w) ->
         let regreads = map rator (dest_list(find_term is_list w)) in
@@ -22,8 +23,8 @@ let GHOST_REGLIST_TAC =
         let ghostvars = map (C (curry mk_var) `:int64`) regnames in
         EVERY(map2 GHOST_INTRO_TAC ghostvars regreads));;
 
-let mlkem_keccak_f1600_x86_mc_4 = define_assert_from_elf
-  "mlkem_keccak_f1600_x86_mc_4" "x86/mlkem/mlkem_keccak_f1600_no_stack.o"
+let mlkem_keccak_f1600_x86_mc_9 = define_assert_from_elf
+  "mlkem_keccak_f1600_x86_mc_9" "x86/mlkem/mlkem_keccak_f1600_no_stack.o"
 [
   0x53;                    (* PUSH (% rbx) *)
   0x55;                    (* PUSH (% rbp) *)
@@ -33,7 +34,6 @@ let mlkem_keccak_f1600_x86_mc_4 = define_assert_from_elf
   0x41; 0x57;              (* PUSH (% r15) *)
   0x48; 0x81; 0xec; 0xd0; 0x00; 0x00; 0x00;
                            (* SUB (% rsp) (Imm32 (word 208)) *)
-  0x49; 0x89; 0xf7;        (* MOV (% r15) (% rsi) *)
   0x48; 0xf7; 0x57; 0x08;  (* NOT (Memop Quadword (%% (rdi,8))) *)
   0x48; 0xf7; 0x57; 0x10;  (* NOT (Memop Quadword (%% (rdi,16))) *)
   0x48; 0xf7; 0x57; 0x40;  (* NOT (Memop Quadword (%% (rdi,64))) *)
@@ -42,7 +42,7 @@ let mlkem_keccak_f1600_x86_mc_4 = define_assert_from_elf
                            (* NOT (Memop Quadword (%% (rdi,136))) *)
   0x48; 0xf7; 0x97; 0xa0; 0x00; 0x00; 0x00;
                            (* NOT (Memop Quadword (%% (rdi,160))) *)
-  0x48; 0x89; 0xe6;        (* MOV (% rsi) (% rsp) *)
+  0x4c; 0x8d; 0x3c; 0x24;  (* LEA (% r15) (%% (rsp,0)) *)
   0x48; 0x8b; 0x87; 0xa0; 0x00; 0x00; 0x00;
                            (* MOV (% rax) (Memop Quadword (%% (rdi,160))) *)
   0x48; 0x8b; 0x9f; 0xa8; 0x00; 0x00; 0x00;
@@ -109,29 +109,29 @@ let mlkem_keccak_f1600_x86_mc_4 = define_assert_from_elf
   0x4d; 0x09; 0xd1;        (* OR (% r9) (% r10) *)
   0x4d; 0x31; 0xc1;        (* XOR (% r9) (% r8) *)
   0x49; 0xc1; 0xc4; 0x0e;  (* ROL (% r12) (Imm8 (word 14)) *)
-  0x4d; 0x33; 0x0f;        (* XOR (% r9) (Memop Quadword (%% (r15,0))) *)
+  0x4c; 0x33; 0x0e;        (* XOR (% r9) (Memop Quadword (%% (rsi,0))) *)
   0x4d; 0x89; 0xe6;        (* MOV (% r14) (% r12) *)
   0x4d; 0x21; 0xdc;        (* AND (% r12) (% r11) *)
-  0x4c; 0x89; 0x0e;        (* MOV (Memop Quadword (%% (rsi,0))) (% r9) *)
+  0x4d; 0x89; 0x0f;        (* MOV (Memop Quadword (%% (r15,0))) (% r9) *)
   0x4d; 0x31; 0xd4;        (* XOR (% r12) (% r10) *)
   0x49; 0xf7; 0xd2;        (* NOT (% r10) *)
-  0x4c; 0x89; 0x66; 0x10;  (* MOV (Memop Quadword (%% (rsi,16))) (% r12) *)
+  0x4d; 0x89; 0x67; 0x10;  (* MOV (Memop Quadword (%% (r15,16))) (% r12) *)
   0x4d; 0x09; 0xda;        (* OR (% r10) (% r11) *)
   0x4c; 0x8b; 0xa7; 0xb0; 0x00; 0x00; 0x00;
                            (* MOV (% r12) (Memop Quadword (%% (rdi,176))) *)
   0x4d; 0x31; 0xea;        (* XOR (% r10) (% r13) *)
-  0x4c; 0x89; 0x56; 0x08;  (* MOV (Memop Quadword (%% (rsi,8))) (% r10) *)
+  0x4d; 0x89; 0x57; 0x08;  (* MOV (Memop Quadword (%% (r15,8))) (% r10) *)
   0x4d; 0x21; 0xc5;        (* AND (% r13) (% r8) *)
   0x4c; 0x8b; 0x4f; 0x48;  (* MOV (% r9) (Memop Quadword (%% (rdi,72))) *)
   0x4d; 0x31; 0xf5;        (* XOR (% r13) (% r14) *)
   0x4c; 0x8b; 0x57; 0x50;  (* MOV (% r10) (Memop Quadword (%% (rdi,80))) *)
-  0x4c; 0x89; 0x6e; 0x20;  (* MOV (Memop Quadword (%% (rsi,32))) (% r13) *)
+  0x4d; 0x89; 0x6f; 0x20;  (* MOV (Memop Quadword (%% (r15,32))) (% r13) *)
   0x4d; 0x09; 0xc6;        (* OR (% r14) (% r8) *)
   0x4c; 0x8b; 0x47; 0x18;  (* MOV (% r8) (Memop Quadword (%% (rdi,24))) *)
   0x4d; 0x31; 0xde;        (* XOR (% r14) (% r11) *)
   0x4c; 0x8b; 0x9f; 0x80; 0x00; 0x00; 0x00;
                            (* MOV (% r11) (Memop Quadword (%% (rdi,128))) *)
-  0x4c; 0x89; 0x76; 0x18;  (* MOV (Memop Quadword (%% (rsi,24))) (% r14) *)
+  0x4d; 0x89; 0x77; 0x18;  (* MOV (Memop Quadword (%% (r15,24))) (% r14) *)
   0x49; 0x31; 0xe8;        (* XOR (% r8) (% rbp) *)
   0x49; 0x31; 0xd4;        (* XOR (% r12) (% rdx) *)
   0x49; 0xc1; 0xc0; 0x1c;  (* ROL (% r8) (Imm8 (word 28)) *)
@@ -145,28 +145,28 @@ let mlkem_keccak_f1600_x86_mc_4 = define_assert_from_elf
   0x4d; 0x09; 0xe0;        (* OR (% r8) (% r12) *)
   0x49; 0xc1; 0xc2; 0x03;  (* ROL (% r10) (Imm8 (word 3)) *)
   0x4d; 0x31; 0xd8;        (* XOR (% r8) (% r11) *)
-  0x4c; 0x89; 0x46; 0x40;  (* MOV (Memop Quadword (%% (rsi,64))) (% r8) *)
+  0x4d; 0x89; 0x47; 0x40;  (* MOV (Memop Quadword (%% (r15,64))) (% r8) *)
   0x4d; 0x89; 0xce;        (* MOV (% r14) (% r9) *)
   0x4d; 0x21; 0xe9;        (* AND (% r9) (% r13) *)
   0x4c; 0x8b; 0x47; 0x08;  (* MOV (% r8) (Memop Quadword (%% (rdi,8))) *)
   0x4d; 0x31; 0xe1;        (* XOR (% r9) (% r12) *)
   0x49; 0xf7; 0xd4;        (* NOT (% r12) *)
-  0x4c; 0x89; 0x4e; 0x48;  (* MOV (Memop Quadword (%% (rsi,72))) (% r9) *)
+  0x4d; 0x89; 0x4f; 0x48;  (* MOV (Memop Quadword (%% (r15,72))) (% r9) *)
   0x4d; 0x09; 0xdc;        (* OR (% r12) (% r11) *)
   0x4c; 0x8b; 0x4f; 0x38;  (* MOV (% r9) (Memop Quadword (%% (rdi,56))) *)
   0x4d; 0x31; 0xd4;        (* XOR (% r12) (% r10) *)
-  0x4c; 0x89; 0x66; 0x38;  (* MOV (Memop Quadword (%% (rsi,56))) (% r12) *)
+  0x4d; 0x89; 0x67; 0x38;  (* MOV (Memop Quadword (%% (r15,56))) (% r12) *)
   0x4d; 0x21; 0xd3;        (* AND (% r11) (% r10) *)
   0x4c; 0x8b; 0xa7; 0xa0; 0x00; 0x00; 0x00;
                            (* MOV (% r12) (Memop Quadword (%% (rdi,160))) *)
   0x4d; 0x31; 0xf3;        (* XOR (% r11) (% r14) *)
-  0x4c; 0x89; 0x5e; 0x30;  (* MOV (Memop Quadword (%% (rsi,48))) (% r11) *)
+  0x4d; 0x89; 0x5f; 0x30;  (* MOV (Memop Quadword (%% (r15,48))) (% r11) *)
   0x4d; 0x09; 0xd6;        (* OR (% r14) (% r10) *)
   0x4c; 0x8b; 0x57; 0x68;  (* MOV (% r10) (Memop Quadword (%% (rdi,104))) *)
   0x4d; 0x31; 0xee;        (* XOR (% r14) (% r13) *)
   0x4c; 0x8b; 0x9f; 0x98; 0x00; 0x00; 0x00;
                            (* MOV (% r11) (Memop Quadword (%% (rdi,152))) *)
-  0x4c; 0x89; 0x76; 0x28;  (* MOV (Memop Quadword (%% (rsi,40))) (% r14) *)
+  0x4d; 0x89; 0x77; 0x28;  (* MOV (Memop Quadword (%% (r15,40))) (% r14) *)
   0x49; 0x31; 0xea;        (* XOR (% r10) (% rbp) *)
   0x49; 0x31; 0xc3;        (* XOR (% r11) (% rax) *)
   0x49; 0xc1; 0xc2; 0x19;  (* ROL (% r10) (Imm8 (word 25)) *)
@@ -181,26 +181,26 @@ let mlkem_keccak_f1600_x86_mc_4 = define_assert_from_elf
   0x49; 0xd1; 0xc0;        (* ROL (% r8) (Imm8 (word 1)) *)
   0x49; 0xf7; 0xd3;        (* NOT (% r11) *)
   0x4d; 0x31; 0xca;        (* XOR (% r10) (% r9) *)
-  0x4c; 0x89; 0x56; 0x58;  (* MOV (Memop Quadword (%% (rsi,88))) (% r10) *)
+  0x4d; 0x89; 0x57; 0x58;  (* MOV (Memop Quadword (%% (r15,88))) (% r10) *)
   0x4d; 0x89; 0xe6;        (* MOV (% r14) (% r12) *)
   0x4d; 0x21; 0xdc;        (* AND (% r12) (% r11) *)
   0x4c; 0x8b; 0x57; 0x58;  (* MOV (% r10) (Memop Quadword (%% (rdi,88))) *)
   0x4d; 0x31; 0xec;        (* XOR (% r12) (% r13) *)
-  0x4c; 0x89; 0x66; 0x60;  (* MOV (Memop Quadword (%% (rsi,96))) (% r12) *)
+  0x4d; 0x89; 0x67; 0x60;  (* MOV (Memop Quadword (%% (r15,96))) (% r12) *)
   0x4d; 0x09; 0xcd;        (* OR (% r13) (% r9) *)
   0x4c; 0x8b; 0xa7; 0xb8; 0x00; 0x00; 0x00;
                            (* MOV (% r12) (Memop Quadword (%% (rdi,184))) *)
   0x4d; 0x31; 0xc5;        (* XOR (% r13) (% r8) *)
-  0x4c; 0x89; 0x6e; 0x50;  (* MOV (Memop Quadword (%% (rsi,80))) (% r13) *)
+  0x4d; 0x89; 0x6f; 0x50;  (* MOV (Memop Quadword (%% (r15,80))) (% r13) *)
   0x4d; 0x21; 0xc1;        (* AND (% r9) (% r8) *)
   0x4d; 0x31; 0xf1;        (* XOR (% r9) (% r14) *)
-  0x4c; 0x89; 0x4e; 0x70;  (* MOV (Memop Quadword (%% (rsi,112))) (% r9) *)
+  0x4d; 0x89; 0x4f; 0x70;  (* MOV (Memop Quadword (%% (r15,112))) (% r9) *)
   0x4d; 0x09; 0xc6;        (* OR (% r14) (% r8) *)
   0x4c; 0x8b; 0x4f; 0x28;  (* MOV (% r9) (Memop Quadword (%% (rdi,40))) *)
   0x4d; 0x31; 0xde;        (* XOR (% r14) (% r11) *)
   0x4c; 0x8b; 0x9f; 0x88; 0x00; 0x00; 0x00;
                            (* MOV (% r11) (Memop Quadword (%% (rdi,136))) *)
-  0x4c; 0x89; 0x76; 0x68;  (* MOV (Memop Quadword (%% (rsi,104))) (% r14) *)
+  0x4d; 0x89; 0x77; 0x68;  (* MOV (Memop Quadword (%% (r15,104))) (% r14) *)
   0x4c; 0x8b; 0x47; 0x20;  (* MOV (% r8) (Memop Quadword (%% (rdi,32))) *)
   0x49; 0x31; 0xca;        (* XOR (% r10) (% rcx) *)
   0x49; 0x31; 0xd3;        (* XOR (% r11) (% rdx) *)
@@ -216,24 +216,24 @@ let mlkem_keccak_f1600_x86_mc_4 = define_assert_from_elf
   0x49; 0xc1; 0xc0; 0x1b;  (* ROL (% r8) (Imm8 (word 27)) *)
   0x49; 0xf7; 0xd3;        (* NOT (% r11) *)
   0x4d; 0x31; 0xca;        (* XOR (% r10) (% r9) *)
-  0x4c; 0x89; 0x96; 0x80; 0x00; 0x00; 0x00;
-                           (* MOV (Memop Quadword (%% (rsi,128))) (% r10) *)
+  0x4d; 0x89; 0x97; 0x80; 0x00; 0x00; 0x00;
+                           (* MOV (Memop Quadword (%% (r15,128))) (% r10) *)
   0x4d; 0x89; 0xe6;        (* MOV (% r14) (% r12) *)
   0x4d; 0x09; 0xdc;        (* OR (% r12) (% r11) *)
   0x4d; 0x31; 0xec;        (* XOR (% r12) (% r13) *)
-  0x4c; 0x89; 0xa6; 0x88; 0x00; 0x00; 0x00;
-                           (* MOV (Memop Quadword (%% (rsi,136))) (% r12) *)
+  0x4d; 0x89; 0xa7; 0x88; 0x00; 0x00; 0x00;
+                           (* MOV (Memop Quadword (%% (r15,136))) (% r12) *)
   0x4d; 0x21; 0xcd;        (* AND (% r13) (% r9) *)
   0x4d; 0x31; 0xc5;        (* XOR (% r13) (% r8) *)
-  0x4c; 0x89; 0x6e; 0x78;  (* MOV (Memop Quadword (%% (rsi,120))) (% r13) *)
+  0x4d; 0x89; 0x6f; 0x78;  (* MOV (Memop Quadword (%% (r15,120))) (% r13) *)
   0x4d; 0x09; 0xc1;        (* OR (% r9) (% r8) *)
   0x4d; 0x31; 0xf1;        (* XOR (% r9) (% r14) *)
-  0x4c; 0x89; 0x8e; 0x98; 0x00; 0x00; 0x00;
-                           (* MOV (Memop Quadword (%% (rsi,152))) (% r9) *)
+  0x4d; 0x89; 0x8f; 0x98; 0x00; 0x00; 0x00;
+                           (* MOV (Memop Quadword (%% (r15,152))) (% r9) *)
   0x4d; 0x21; 0xf0;        (* AND (% r8) (% r14) *)
   0x4d; 0x31; 0xd8;        (* XOR (% r8) (% r11) *)
-  0x4c; 0x89; 0x86; 0x90; 0x00; 0x00; 0x00;
-                           (* MOV (Memop Quadword (%% (rsi,144))) (% r8) *)
+  0x4d; 0x89; 0x87; 0x90; 0x00; 0x00; 0x00;
+                           (* MOV (Memop Quadword (%% (r15,144))) (% r8) *)
   0x48; 0x33; 0x57; 0x10;  (* XOR (% rdx) (Memop Quadword (%% (rdi,16))) *)
   0x48; 0x33; 0x6f; 0x40;  (* XOR (% rbp) (Memop Quadword (%% (rdi,64))) *)
   0x48; 0xc1; 0xc2; 0x3e;  (* ROL (% rdx) (Imm8 (word 62)) *)
@@ -243,7 +243,7 @@ let mlkem_keccak_f1600_x86_mc_4 = define_assert_from_elf
   0x48; 0x33; 0x47; 0x70;  (* XOR (% rax) (Memop Quadword (%% (rdi,112))) *)
   0x48; 0xc1; 0xc1; 0x02;  (* ROL (% rcx) (Imm8 (word 2)) *)
   0x48; 0x33; 0x5f; 0x78;  (* XOR (% rbx) (Memop Quadword (%% (rdi,120))) *)
-  0x48; 0x87; 0xf7;        (* XCHG (% rsi) (% rdi) *)
+  0x4c; 0x87; 0xff;        (* XCHG (% r15) (% rdi) *)
   0x48; 0xc1; 0xc0; 0x27;  (* ROL (% rax) (Imm8 (word 39)) *)
   0x48; 0xc1; 0xc3; 0x29;  (* ROL (% rbx) (Imm8 (word 41)) *)
   0x49; 0x89; 0xd5;        (* MOV (% r13) (% rdx) *)
@@ -271,7 +271,7 @@ let mlkem_keccak_f1600_x86_mc_4 = define_assert_from_elf
                            (* MOV (Memop Quadword (%% (rdi,168))) (% rbx) *)
   0x48; 0x89; 0xd5;        (* MOV (% rbp) (% rdx) *)
   0x4c; 0x89; 0xea;        (* MOV (% rdx) (% r13) *)
-  0x49; 0x83; 0xc7; 0x08;  (* ADD (% r15) (Imm8 (word 8)) *)
+  0x48; 0x8d; 0x76; 0x08;  (* LEA (% rsi) (%% (rsi,8)) *)
   0x4c; 0x8b; 0x07;        (* MOV (% r8) (Memop Quadword (%% (rdi,0))) *)
   0x4c; 0x8b; 0x4f; 0x30;  (* MOV (% r9) (Memop Quadword (%% (rdi,48))) *)
   0x4c; 0x8b; 0x57; 0x60;  (* MOV (% r10) (Memop Quadword (%% (rdi,96))) *)
@@ -324,29 +324,29 @@ let mlkem_keccak_f1600_x86_mc_4 = define_assert_from_elf
   0x4d; 0x09; 0xd1;        (* OR (% r9) (% r10) *)
   0x4d; 0x31; 0xc1;        (* XOR (% r9) (% r8) *)
   0x49; 0xc1; 0xc4; 0x0e;  (* ROL (% r12) (Imm8 (word 14)) *)
-  0x4d; 0x33; 0x0f;        (* XOR (% r9) (Memop Quadword (%% (r15,0))) *)
+  0x4c; 0x33; 0x0e;        (* XOR (% r9) (Memop Quadword (%% (rsi,0))) *)
   0x4d; 0x89; 0xe6;        (* MOV (% r14) (% r12) *)
   0x4d; 0x21; 0xdc;        (* AND (% r12) (% r11) *)
-  0x4c; 0x89; 0x0e;        (* MOV (Memop Quadword (%% (rsi,0))) (% r9) *)
+  0x4d; 0x89; 0x0f;        (* MOV (Memop Quadword (%% (r15,0))) (% r9) *)
   0x4d; 0x31; 0xd4;        (* XOR (% r12) (% r10) *)
   0x49; 0xf7; 0xd2;        (* NOT (% r10) *)
-  0x4c; 0x89; 0x66; 0x10;  (* MOV (Memop Quadword (%% (rsi,16))) (% r12) *)
+  0x4d; 0x89; 0x67; 0x10;  (* MOV (Memop Quadword (%% (r15,16))) (% r12) *)
   0x4d; 0x09; 0xda;        (* OR (% r10) (% r11) *)
   0x4c; 0x8b; 0xa7; 0xb0; 0x00; 0x00; 0x00;
                            (* MOV (% r12) (Memop Quadword (%% (rdi,176))) *)
   0x4d; 0x31; 0xea;        (* XOR (% r10) (% r13) *)
-  0x4c; 0x89; 0x56; 0x08;  (* MOV (Memop Quadword (%% (rsi,8))) (% r10) *)
+  0x4d; 0x89; 0x57; 0x08;  (* MOV (Memop Quadword (%% (r15,8))) (% r10) *)
   0x4d; 0x21; 0xc5;        (* AND (% r13) (% r8) *)
   0x4c; 0x8b; 0x4f; 0x48;  (* MOV (% r9) (Memop Quadword (%% (rdi,72))) *)
   0x4d; 0x31; 0xf5;        (* XOR (% r13) (% r14) *)
   0x4c; 0x8b; 0x57; 0x50;  (* MOV (% r10) (Memop Quadword (%% (rdi,80))) *)
-  0x4c; 0x89; 0x6e; 0x20;  (* MOV (Memop Quadword (%% (rsi,32))) (% r13) *)
+  0x4d; 0x89; 0x6f; 0x20;  (* MOV (Memop Quadword (%% (r15,32))) (% r13) *)
   0x4d; 0x09; 0xc6;        (* OR (% r14) (% r8) *)
   0x4c; 0x8b; 0x47; 0x18;  (* MOV (% r8) (Memop Quadword (%% (rdi,24))) *)
   0x4d; 0x31; 0xde;        (* XOR (% r14) (% r11) *)
   0x4c; 0x8b; 0x9f; 0x80; 0x00; 0x00; 0x00;
                            (* MOV (% r11) (Memop Quadword (%% (rdi,128))) *)
-  0x4c; 0x89; 0x76; 0x18;  (* MOV (Memop Quadword (%% (rsi,24))) (% r14) *)
+  0x4d; 0x89; 0x77; 0x18;  (* MOV (Memop Quadword (%% (r15,24))) (% r14) *)
   0x49; 0x31; 0xe8;        (* XOR (% r8) (% rbp) *)
   0x49; 0x31; 0xd4;        (* XOR (% r12) (% rdx) *)
   0x49; 0xc1; 0xc0; 0x1c;  (* ROL (% r8) (Imm8 (word 28)) *)
@@ -360,28 +360,28 @@ let mlkem_keccak_f1600_x86_mc_4 = define_assert_from_elf
   0x4d; 0x09; 0xe0;        (* OR (% r8) (% r12) *)
   0x49; 0xc1; 0xc2; 0x03;  (* ROL (% r10) (Imm8 (word 3)) *)
   0x4d; 0x31; 0xd8;        (* XOR (% r8) (% r11) *)
-  0x4c; 0x89; 0x46; 0x40;  (* MOV (Memop Quadword (%% (rsi,64))) (% r8) *)
+  0x4d; 0x89; 0x47; 0x40;  (* MOV (Memop Quadword (%% (r15,64))) (% r8) *)
   0x4d; 0x89; 0xce;        (* MOV (% r14) (% r9) *)
   0x4d; 0x21; 0xe9;        (* AND (% r9) (% r13) *)
   0x4c; 0x8b; 0x47; 0x08;  (* MOV (% r8) (Memop Quadword (%% (rdi,8))) *)
   0x4d; 0x31; 0xe1;        (* XOR (% r9) (% r12) *)
   0x49; 0xf7; 0xd4;        (* NOT (% r12) *)
-  0x4c; 0x89; 0x4e; 0x48;  (* MOV (Memop Quadword (%% (rsi,72))) (% r9) *)
+  0x4d; 0x89; 0x4f; 0x48;  (* MOV (Memop Quadword (%% (r15,72))) (% r9) *)
   0x4d; 0x09; 0xdc;        (* OR (% r12) (% r11) *)
   0x4c; 0x8b; 0x4f; 0x38;  (* MOV (% r9) (Memop Quadword (%% (rdi,56))) *)
   0x4d; 0x31; 0xd4;        (* XOR (% r12) (% r10) *)
-  0x4c; 0x89; 0x66; 0x38;  (* MOV (Memop Quadword (%% (rsi,56))) (% r12) *)
+  0x4d; 0x89; 0x67; 0x38;  (* MOV (Memop Quadword (%% (r15,56))) (% r12) *)
   0x4d; 0x21; 0xd3;        (* AND (% r11) (% r10) *)
   0x4c; 0x8b; 0xa7; 0xa0; 0x00; 0x00; 0x00;
                            (* MOV (% r12) (Memop Quadword (%% (rdi,160))) *)
   0x4d; 0x31; 0xf3;        (* XOR (% r11) (% r14) *)
-  0x4c; 0x89; 0x5e; 0x30;  (* MOV (Memop Quadword (%% (rsi,48))) (% r11) *)
+  0x4d; 0x89; 0x5f; 0x30;  (* MOV (Memop Quadword (%% (r15,48))) (% r11) *)
   0x4d; 0x09; 0xd6;        (* OR (% r14) (% r10) *)
   0x4c; 0x8b; 0x57; 0x68;  (* MOV (% r10) (Memop Quadword (%% (rdi,104))) *)
   0x4d; 0x31; 0xee;        (* XOR (% r14) (% r13) *)
   0x4c; 0x8b; 0x9f; 0x98; 0x00; 0x00; 0x00;
                            (* MOV (% r11) (Memop Quadword (%% (rdi,152))) *)
-  0x4c; 0x89; 0x76; 0x28;  (* MOV (Memop Quadword (%% (rsi,40))) (% r14) *)
+  0x4d; 0x89; 0x77; 0x28;  (* MOV (Memop Quadword (%% (r15,40))) (% r14) *)
   0x49; 0x31; 0xea;        (* XOR (% r10) (% rbp) *)
   0x49; 0x31; 0xc3;        (* XOR (% r11) (% rax) *)
   0x49; 0xc1; 0xc2; 0x19;  (* ROL (% r10) (Imm8 (word 25)) *)
@@ -396,26 +396,26 @@ let mlkem_keccak_f1600_x86_mc_4 = define_assert_from_elf
   0x49; 0xd1; 0xc0;        (* ROL (% r8) (Imm8 (word 1)) *)
   0x49; 0xf7; 0xd3;        (* NOT (% r11) *)
   0x4d; 0x31; 0xca;        (* XOR (% r10) (% r9) *)
-  0x4c; 0x89; 0x56; 0x58;  (* MOV (Memop Quadword (%% (rsi,88))) (% r10) *)
+  0x4d; 0x89; 0x57; 0x58;  (* MOV (Memop Quadword (%% (r15,88))) (% r10) *)
   0x4d; 0x89; 0xe6;        (* MOV (% r14) (% r12) *)
   0x4d; 0x21; 0xdc;        (* AND (% r12) (% r11) *)
   0x4c; 0x8b; 0x57; 0x58;  (* MOV (% r10) (Memop Quadword (%% (rdi,88))) *)
   0x4d; 0x31; 0xec;        (* XOR (% r12) (% r13) *)
-  0x4c; 0x89; 0x66; 0x60;  (* MOV (Memop Quadword (%% (rsi,96))) (% r12) *)
+  0x4d; 0x89; 0x67; 0x60;  (* MOV (Memop Quadword (%% (r15,96))) (% r12) *)
   0x4d; 0x09; 0xcd;        (* OR (% r13) (% r9) *)
   0x4c; 0x8b; 0xa7; 0xb8; 0x00; 0x00; 0x00;
                            (* MOV (% r12) (Memop Quadword (%% (rdi,184))) *)
   0x4d; 0x31; 0xc5;        (* XOR (% r13) (% r8) *)
-  0x4c; 0x89; 0x6e; 0x50;  (* MOV (Memop Quadword (%% (rsi,80))) (% r13) *)
+  0x4d; 0x89; 0x6f; 0x50;  (* MOV (Memop Quadword (%% (r15,80))) (% r13) *)
   0x4d; 0x21; 0xc1;        (* AND (% r9) (% r8) *)
   0x4d; 0x31; 0xf1;        (* XOR (% r9) (% r14) *)
-  0x4c; 0x89; 0x4e; 0x70;  (* MOV (Memop Quadword (%% (rsi,112))) (% r9) *)
+  0x4d; 0x89; 0x4f; 0x70;  (* MOV (Memop Quadword (%% (r15,112))) (% r9) *)
   0x4d; 0x09; 0xc6;        (* OR (% r14) (% r8) *)
   0x4c; 0x8b; 0x4f; 0x28;  (* MOV (% r9) (Memop Quadword (%% (rdi,40))) *)
   0x4d; 0x31; 0xde;        (* XOR (% r14) (% r11) *)
   0x4c; 0x8b; 0x9f; 0x88; 0x00; 0x00; 0x00;
                            (* MOV (% r11) (Memop Quadword (%% (rdi,136))) *)
-  0x4c; 0x89; 0x76; 0x68;  (* MOV (Memop Quadword (%% (rsi,104))) (% r14) *)
+  0x4d; 0x89; 0x77; 0x68;  (* MOV (Memop Quadword (%% (r15,104))) (% r14) *)
   0x4c; 0x8b; 0x47; 0x20;  (* MOV (% r8) (Memop Quadword (%% (rdi,32))) *)
   0x49; 0x31; 0xca;        (* XOR (% r10) (% rcx) *)
   0x49; 0x31; 0xd3;        (* XOR (% r11) (% rdx) *)
@@ -431,24 +431,24 @@ let mlkem_keccak_f1600_x86_mc_4 = define_assert_from_elf
   0x49; 0xc1; 0xc0; 0x1b;  (* ROL (% r8) (Imm8 (word 27)) *)
   0x49; 0xf7; 0xd3;        (* NOT (% r11) *)
   0x4d; 0x31; 0xca;        (* XOR (% r10) (% r9) *)
-  0x4c; 0x89; 0x96; 0x80; 0x00; 0x00; 0x00;
-                           (* MOV (Memop Quadword (%% (rsi,128))) (% r10) *)
+  0x4d; 0x89; 0x97; 0x80; 0x00; 0x00; 0x00;
+                           (* MOV (Memop Quadword (%% (r15,128))) (% r10) *)
   0x4d; 0x89; 0xe6;        (* MOV (% r14) (% r12) *)
   0x4d; 0x09; 0xdc;        (* OR (% r12) (% r11) *)
   0x4d; 0x31; 0xec;        (* XOR (% r12) (% r13) *)
-  0x4c; 0x89; 0xa6; 0x88; 0x00; 0x00; 0x00;
-                           (* MOV (Memop Quadword (%% (rsi,136))) (% r12) *)
+  0x4d; 0x89; 0xa7; 0x88; 0x00; 0x00; 0x00;
+                           (* MOV (Memop Quadword (%% (r15,136))) (% r12) *)
   0x4d; 0x21; 0xcd;        (* AND (% r13) (% r9) *)
   0x4d; 0x31; 0xc5;        (* XOR (% r13) (% r8) *)
-  0x4c; 0x89; 0x6e; 0x78;  (* MOV (Memop Quadword (%% (rsi,120))) (% r13) *)
+  0x4d; 0x89; 0x6f; 0x78;  (* MOV (Memop Quadword (%% (r15,120))) (% r13) *)
   0x4d; 0x09; 0xc1;        (* OR (% r9) (% r8) *)
   0x4d; 0x31; 0xf1;        (* XOR (% r9) (% r14) *)
-  0x4c; 0x89; 0x8e; 0x98; 0x00; 0x00; 0x00;
-                           (* MOV (Memop Quadword (%% (rsi,152))) (% r9) *)
+  0x4d; 0x89; 0x8f; 0x98; 0x00; 0x00; 0x00;
+                           (* MOV (Memop Quadword (%% (r15,152))) (% r9) *)
   0x4d; 0x21; 0xf0;        (* AND (% r8) (% r14) *)
   0x4d; 0x31; 0xd8;        (* XOR (% r8) (% r11) *)
-  0x4c; 0x89; 0x86; 0x90; 0x00; 0x00; 0x00;
-                           (* MOV (Memop Quadword (%% (rsi,144))) (% r8) *)
+  0x4d; 0x89; 0x87; 0x90; 0x00; 0x00; 0x00;
+                           (* MOV (Memop Quadword (%% (r15,144))) (% r8) *)
   0x48; 0x33; 0x57; 0x10;  (* XOR (% rdx) (Memop Quadword (%% (rdi,16))) *)
   0x48; 0x33; 0x6f; 0x40;  (* XOR (% rbp) (Memop Quadword (%% (rdi,64))) *)
   0x48; 0xc1; 0xc2; 0x3e;  (* ROL (% rdx) (Imm8 (word 62)) *)
@@ -458,7 +458,7 @@ let mlkem_keccak_f1600_x86_mc_4 = define_assert_from_elf
   0x48; 0x33; 0x47; 0x70;  (* XOR (% rax) (Memop Quadword (%% (rdi,112))) *)
   0x48; 0xc1; 0xc1; 0x02;  (* ROL (% rcx) (Imm8 (word 2)) *)
   0x48; 0x33; 0x5f; 0x78;  (* XOR (% rbx) (Memop Quadword (%% (rdi,120))) *)
-  0x48; 0x87; 0xf7;        (* XCHG (% rsi) (% rdi) *)
+  0x4c; 0x87; 0xff;        (* XCHG (% r15) (% rdi) *)
   0x48; 0xc1; 0xc0; 0x27;  (* ROL (% rax) (Imm8 (word 39)) *)
   0x48; 0xc1; 0xc3; 0x29;  (* ROL (% rbx) (Imm8 (word 41)) *)
   0x49; 0x89; 0xd5;        (* MOV (% r13) (% rdx) *)
@@ -486,13 +486,15 @@ let mlkem_keccak_f1600_x86_mc_4 = define_assert_from_elf
                            (* MOV (Memop Quadword (%% (rdi,168))) (% rbx) *)
   0x48; 0x89; 0xd5;        (* MOV (% rbp) (% rdx) *)
   0x4c; 0x89; 0xea;        (* MOV (% rdx) (% r13) *)
-  0x49; 0x83; 0xc7; 0x08;  (* ADD (% r15) (Imm8 (word 8)) *)
+  0x48; 0x8d; 0x76; 0x08;  (* LEA (% rsi) (%% (rsi,8)) *)
   0x4c; 0x8b; 0x84; 0x24; 0xc8; 0x00; 0x00; 0x00;
                            (* MOV (% r8) (Memop Quadword (%% (rsp,200))) *)
   0x49; 0x83; 0xc0; 0x02;  (* ADD (% r8) (Imm8 (word 2)) *)
   0x49; 0x83; 0xf8; 0x18;  (* CMP (% r8) (Imm8 (word 24)) *)
   0x0f; 0x85; 0x2a; 0xfa; 0xff; 0xff;
                            (* JNE (Imm32 (word 4294965802)) *)
+  0x48; 0x8d; 0xb6; 0x40; 0xff; 0xff; 0xff;
+                           (* LEA (% rsi) (%% (rsi,18446744073709551424)) *)
   0x48; 0xf7; 0x57; 0x08;  (* NOT (Memop Quadword (%% (rdi,8))) *)
   0x48; 0xf7; 0x57; 0x10;  (* NOT (Memop Quadword (%% (rdi,16))) *)
   0x48; 0xf7; 0x57; 0x40;  (* NOT (Memop Quadword (%% (rdi,64))) *)
@@ -503,7 +505,7 @@ let mlkem_keccak_f1600_x86_mc_4 = define_assert_from_elf
                            (* NOT (Memop Quadword (%% (rdi,160))) *)
   0x48; 0x81; 0xc4; 0xd0; 0x00; 0x00; 0x00;
                            (* ADD (% rsp) (Imm32 (word 208)) *)
-  0x41; 0x5f;              (* POP (% r15) *)
+  0x5e;                    (* POP (% rsi) *)
   0x41; 0x5e;              (* POP (% r14) *)
   0x41; 0x5d;              (* POP (% r13) *)
   0x41; 0x5c;              (* POP (% r12) *)
@@ -512,8 +514,9 @@ let mlkem_keccak_f1600_x86_mc_4 = define_assert_from_elf
   0xc3                     (* RET *)
 ];;
 
- let MLKEM_KECCAK_F1600_EXEC_4 = X86_MK_EXEC_RULE mlkem_keccak_f1600_x86_mc_4;;
+ 
 
+let MLKEM_KECCAK_F1600_EXEC_9 = X86_MK_EXEC_RULE mlkem_keccak_f1600_x86_mc_9;;
 
  let wordlist_from_memory = define
  `wordlist_from_memory(bitstate_in,0) s = [] /\
@@ -541,14 +544,14 @@ let WORDLIST_FROM_MEMORY_CONV =
 
   let MLKEM_KECCAK_F1600_SPEC = prove(
   `forall rc_pointer:int64 pc:num stackpointer:int64 bitstate_in:int64 A.
-  nonoverlapping_modulo (2 EXP 64) (pc, LENGTH mlkem_keccak_f1600_x86_mc_4) (val  (word_add stackpointer (word 0)), 264) /\
-  nonoverlapping_modulo (2 EXP 64) (pc, LENGTH mlkem_keccak_f1600_x86_mc_4) (val bitstate_in, 200) /\
-  nonoverlapping_modulo (2 EXP 64) (pc, LENGTH mlkem_keccak_f1600_x86_mc_4) (val rc_pointer, 192) /\
+  nonoverlapping_modulo (2 EXP 64) (pc, LENGTH mlkem_keccak_f1600_x86_mc_9) (val  stackpointer, 264) /\
+  nonoverlapping_modulo (2 EXP 64) (pc, LENGTH mlkem_keccak_f1600_x86_mc_9) (val bitstate_in, 200) /\
+  nonoverlapping_modulo (2 EXP 64) (pc, LENGTH mlkem_keccak_f1600_x86_mc_9) (val rc_pointer, 192) /\
 
   nonoverlapping_modulo (2 EXP 64) (val bitstate_in,200) (val rc_pointer,192) /\
-  nonoverlapping_modulo (2 EXP 64) (val bitstate_in,200) (val (word_add stackpointer (word 0)), 264) /\
+  nonoverlapping_modulo (2 EXP 64) (val bitstate_in,200) (val stackpointer, 264) /\
 
-  nonoverlapping_modulo (2 EXP 64) (val (word_add stackpointer (word 0)), 264) (val rc_pointer,192)
+  nonoverlapping_modulo (2 EXP 64) (val stackpointer, 264) (val rc_pointer,192)
 
   // RSI is used to pass the rc bitstate_out address, however, it is later assigned as a bitsate' 
   // bitstate_in/bitstate_in' are used as input/output value for the keccak loop
@@ -557,9 +560,10 @@ let WORDLIST_FROM_MEMORY_CONV =
   // the output of the previous interaiton will serve as an input to the following iteration
       ==> ensures x86
   // Precondition
-  (\s. bytes_loaded s (word pc) mlkem_keccak_f1600_x86_mc_4 /\
-       read RIP s = word (pc + 17) /\
+  (\s. bytes_loaded s (word pc) mlkem_keccak_f1600_x86_mc_9 /\
+       read RIP s = word (pc + 0x11) /\
        read RSP s = stackpointer /\
+       read RSI s = rc_pointer /\
        C_ARGUMENTS [bitstate_in; rc_pointer] s /\
                 wordlist_from_memory(rc_pointer,24) s = rc_table /\
                 wordlist_from_memory(bitstate_in,25) s = A
@@ -575,12 +579,12 @@ let WORDLIST_FROM_MEMORY_CONV =
 
   REWRITE_TAC[SOME_FLAGS] THEN
   MAP_EVERY X_GEN_TAC [`rc_pointer:int64`; `pc:num`] THEN
-  REWRITE_TAC [(REWRITE_CONV [mlkem_keccak_f1600_x86_mc_4] THENC LENGTH_CONV) `LENGTH mlkem_keccak_f1600_x86_mc_4`] THEN
+  REWRITE_TAC [(REWRITE_CONV [mlkem_keccak_f1600_x86_mc_9] THENC LENGTH_CONV) `LENGTH mlkem_keccak_f1600_x86_mc_9`] THEN
 
     MAP_EVERY X_GEN_TAC [`stackpointer:int64`;`bitstate_in:int64`;`A:int64 list`] THEN
 
 
-  REWRITE_TAC[fst MLKEM_KECCAK_F1600_EXEC_4] THEN
+  REWRITE_TAC[fst MLKEM_KECCAK_F1600_EXEC_9] THEN
   REWRITE_TAC[MAYCHANGE_REGS_AND_FLAGS_PERMITTED_BY_ABI; C_ARGUMENTS;
               ALL; ALLPAIRS; NONOVERLAPPING_CLAUSES] THEN
   DISCH_THEN(REPEAT_TCL CONJUNCTS_THEN ASSUME_TAC) THEN
@@ -593,19 +597,22 @@ let WORDLIST_FROM_MEMORY_CONV =
               true;  false; false; false; false]
               (wordlist_from_memory(bitstate_in,25) s) = keccak (2*i) A  *)
 
-  
+
   REPEAT STRIP_TAC THEN
+
+            (* read R15 s = word_add rc_pointer (word (16 * i)) /\ *)
 
     ENSURES_WHILE_PAUP_TAC
     `0` (* loop_body begin number *)
     `12` (* loop_body end number *)
-    `pc + 0x5f` (* loop body start PC *)
-    `pc + 0x62f` (* loop backedge branch PC -- including the jmp *) 
+    `pc + 0x5d` (* loop body start PC *)
+    `pc + 0x62d` (* loop backedge branch PC -- including the jmp *) 
     `\i s. // loop invariant at the end of the iteration
             (read R8 s = word (2*i) /\
             read RDI s = bitstate_in /\
             read RSP s = stackpointer /\
-            read RSI s = stackpointer /\
+            read R15 s = stackpointer /\
+            read RSI s = word_add rc_pointer (word (16 * i)) /\
             wordlist_from_memory(rc_pointer,24) s = rc_table /\
             wordlist_from_memory(bitstate_in,25) s = MAP2 (\(x:bool) (y:(64)word). (if x then (word_not y) else y)) (
               [false; true;  true;  false; false; 
@@ -623,117 +630,262 @@ let WORDLIST_FROM_MEMORY_CONV =
 
           (* program_begin until loop_entry *)
 
-          REWRITE_TAC[rc_table; CONS_11; GSYM CONJ_ASSOC; 
-                        WORDLIST_FROM_MEMORY_CONV `wordlist_from_memory(rc_pointer,24) s:int64 list`; 
-                        WORDLIST_FROM_MEMORY_CONV `wordlist_from_memory(bitstate_in,25) s:int64 list`] THEN
+          REWRITE_TAC[rc_table; CONS_11; GSYM CONJ_ASSOC; WORDLIST_FROM_MEMORY_CONV `wordlist_from_memory(rc_pointer,24) s:int64 list`; WORDLIST_FROM_MEMORY_CONV `wordlist_from_memory(bitstate_in,25) s:int64 list`] THEN
           ENSURES_INIT_TAC "s0" THEN
           BIGNUM_DIGITIZE_TAC "A_" `read (memory :> bytes (bitstate_in,8 * 25)) s0` THEN
-
-          ASM_REWRITE_TAC[] THEN REPEAT DISCH_TAC THEN
-
-          ASM_REWRITE_TAC[WORD_ADD_0] THEN REPEAT STRIP_TAC THEN
-
-          (* X86_STEPS_TAC MLKEM_KECCAK_F1600_EXEC_4 (1--13) THEN *)
-
-          X86_STEPS_TAC MLKEM_KECCAK_F1600_EXEC_4 (1--14) THEN
-
+          ASM_REWRITE_TAC[] THEN
+          X86_STEPS_TAC MLKEM_KECCAK_F1600_EXEC_9 (1--13) THEN
           ENSURES_FINAL_STATE_TAC THEN ASM_REWRITE_TAC[] THEN
-
-       
-
 
           (* In progress; Works until HERE depending on addresses in the loop invariant*)
           REPEAT CONJ_TAC THENL 
           [
                 CONV_TAC WORD_RULE;
 
-                   GEN_REWRITE_TAC (RAND_CONV o ONCE_DEPTH_CONV)
-       [ARITH_RULE `2 * 1 = (0 + 1) + 1`] THEN
+                 CONV_TAC WORD_RULE;
+
 
                 EXPAND_TAC "A" THEN
                 CHANGED_TAC(PURE_ONCE_REWRITE_TAC[ARITH_RULE `2 * 0 = 0`]) THEN
 
                 CHANGED_TAC(REWRITE_TAC[keccak]) THEN 
-                CHANGED_TAC(REWRITE_TAC[MAP2;CONS_11]);
+                CHANGED_TAC(REWRITE_TAC[MAP2]);
           ]
 
-          REPEAT STRIP_TAC THEN
 
+          CHANGED_TAC(X_GEN_TAC `i:num`) THEN 
+           CHANGED_TAC(STRIP_TAC) THEN 
+          CHANGED_TAC(VAL_INT64_TAC `i:num`) THEN
+
+          CHANGED_TAC(MAP_EVERY VAL_INT64_TAC [`i:num`; `2 * i`; `2 * i + 1`]) THEN
+
+            GHOST_INTRO_TAC `init_rax:int64` `read RAX` THEN
+          GHOST_INTRO_TAC `init_rbx:int64` `read RBX` THEN
+          GHOST_INTRO_TAC `init_rcx:int64` `read RCX` THEN
+          GHOST_INTRO_TAC `init_rdx:int64` `read RDX` THEN
+          GHOST_INTRO_TAC `init_rbp:int64` `read RBP` THEN
+          GHOST_INTRO_TAC `init_rsi:int64` `read RSI` THEN
+          GHOST_INTRO_TAC `init_r15:int64` `read R15` THEN
+          GHOST_INTRO_TAC `init_r8:int64` `read R8` THEN
+
+          (* REPEAT STRIP_TAC THEN *)
+
+
+(* 
           GHOST_INTRO_TAC `init_rax:int64` `read RAX` THEN
           GHOST_INTRO_TAC `init_rbx:int64` `read RBX` THEN
           GHOST_INTRO_TAC `init_rcx:int64` `read RCX` THEN
           GHOST_INTRO_TAC `init_rdx:int64` `read RDX` THEN
           GHOST_INTRO_TAC `init_rbp:int64` `read RBP` THEN
-          GHOST_INTRO_TAC `init_r8:int64` `read R8` THEN
-          GHOST_INTRO_TAC `init_r15:int64` `read R15` THEN
-          GHOST_INTRO_TAC `init_rdi:int64` `read RDI` THEN
           GHOST_INTRO_TAC `init_rsi:int64` `read RSI` THEN
+          GHOST_INTRO_TAC `init_r15:int64` `read R15` THEN
+          GHOST_INTRO_TAC `init_r8:int64` `read R8` THEN *)
 
-          REWRITE_TAC[rc_table; CONS_11; GSYM CONJ_ASSOC; 
-                   WORDLIST_FROM_MEMORY_CONV `wordlist_from_memory(rc_pointer,24) s:int64 list`;
-                   WORDLIST_FROM_MEMORY_CONV `wordlist_from_memory(bitstate_in,25) s:int64 list`] THEN
+
+        
+
+           (* GHOST_INTRO_TAC `init_rsi:int64` `read RSI` THEN *)
+
+
+        REWRITE_TAC[rc_table; CONS_11; GSYM CONJ_ASSOC; WORDLIST_FROM_MEMORY_CONV `wordlist_from_memory(rc_pointer,24) s:int64 list`; WORDLIST_FROM_MEMORY_CONV `wordlist_from_memory(bitstate_in,25) s:int64 list`] THEN
           ENSURES_INIT_TAC "s0" THEN
-          BIGNUM_DIGITIZE_TAC "A_" `read (memory :> bytes (bitstate_in,8 * 25)) s0` THEN 
-
-          
-          ASM_REWRITE_TAC[] THEN 
-          REPEAT DISCH_TAC THEN
-
-          ASM_REWRITE_TAC[] THEN REPEAT STRIP_TAC THEN
-
-                X86_STEPS_TAC MLKEM_KECCAK_F1600_EXEC_4 (1--1) THEN
-                X86_STEPS_TAC MLKEM_KECCAK_F1600_EXEC_4 (2--10) THEN
-                X86_STEPS_TAC MLKEM_KECCAK_F1600_EXEC_4 (11--20) THEN
-
-                 X86_STEPS_TAC MLKEM_KECCAK_F1600_EXEC_4 (21--30) THEN
-                 X86_VSTEPS_TAC MLKEM_KECCAK_F1600_EXEC_4 (31--40) THEN
-                  X86_STEPS_TAC MLKEM_KECCAK_F1600_EXEC_4 (41--50) THEN
-
-                  X86_STEPS_TAC MLKEM_KECCAK_F1600_EXEC_4 (51--52) THEN
 
 
-                X86_STEPS_TAC MLKEM_KECCAK_F1600_EXEC_4 (53--53) THEN
-                X86_STEPS_TAC MLKEM_KECCAK_F1600_EXEC_4 (54--55) THEN
-                X86_STEPS_TAC MLKEM_KECCAK_F1600_EXEC_4 (56--56) THEN
-                X86_STEPS_TAC MLKEM_KECCAK_F1600_EXEC_4 (57--61) THEN
+     
 
-                X86_STEPS_TAC MLKEM_KECCAK_F1600_EXEC_4 (62--202) THEN
+          BIGNUM_DIGITIZE_TAC "A_" `read (memory :> bytes (bitstate_in,8 * 25)) s0` THEN
 
-                X86_STEPS_TAC MLKEM_KECCAK_F1600_EXEC_4 (203--203) THEN
+ (* !!!! COND_CASES_TAC
+ SIMPLE_ARITH_TAC
 
-                X86_STEPS_TAC MLKEM_KECCAK_F1600_EXEC_4 (204--206) THEN
-
-                X86_STEPS_TAC MLKEM_KECCAK_F1600_EXEC_4 (207--210) THEN
-
-                    X86_STEPS_TAC MLKEM_KECCAK_F1600_EXEC_4 (211--215) THEN
-
-                    X86_STEPS_TAC MLKEM_KECCAK_F1600_EXEC_4 (216--221) THEN
+ ASM_ARITH_TAC, but much faster *)
 
 
-                     X86_STEPS_TAC MLKEM_KECCAK_F1600_EXEC_4 (222--223) THEN
+          SUBGOAL_THEN
+     `read (memory :> bytes64 (word_add rc_pointer (word(8 * i)))) s0 =
+      EL i rc_table /\
+      read (memory :> bytes64 (word_add rc_pointer (word(2 * 8 * i)))) s0 =
+      EL (2 * i) rc_table /\
+      read (memory :> bytes64 (word_add rc_pointer (word(16 * i)))) s0 =
+      EL (2 * i) rc_table /\
+      read (memory :> bytes64 (word_add (word_add rc_pointer (word(16 * i))) (word(8)))) s0 =
+      EL (2 * i + 1) rc_table`
+      ASSUME_TAC THENL
+     
+     
+      [UNDISCH_TAC `i < 12` THEN SPEC_TAC(`i:num`,`i:num`) THEN
+      CONV_TAC EXPAND_CASES_CONV THEN
+      REWRITE_TAC[WORD_ADD_ASSOC_CONSTS] THEN 
 
 
+      CONV_TAC(DEPTH_CONV WORD_NUM_RED_CONV) THEN
+      ASM_REWRITE_TAC[rc_table; WORD_ADD_0] THEN
+      (* REWRITE_TAC[ARITH_RULE`2*11+1 = 23`] THEN *)
+      CONV_TAC(ONCE_DEPTH_CONV EL_CONV) THEN 
 
 
- X86_STEPS_TAC MLKEM_KECCAK_F1600_EXEC_4 (207--210) THEN
+(* REWRITE_TAC[] THEN FAIL_TAC THEN *)
 
-  X86_STEPS_TAC MLKEM_KECCAK_F1600_EXEC_4 (211--220) THEN
 
-   X86_STEPS_TAC MLKEM_KECCAK_F1600_EXEC_4 (221--230) THEN
-      X86_STEPS_TAC MLKEM_KECCAK_F1600_EXEC_4 (221--230) THEN
+      REWRITE_TAC[];
+      ALL_TAC] THEN
+
+
+      X86_STEPS_TAC MLKEM_KECCAK_F1600_EXEC_9 (1--394) THEN
 
 
 
-  ENSURES_FINAL_STATE_TAC THEN ASM_REWRITE_TAC[] THEN
-          
-            REPEAT CONJ_TAC THENL [
+
+
+
+
+
+      ENSURES_FINAL_STATE_TAC THEN 
+      ASM_REWRITE_TAC[] THEN
+
+      
+      REWRITE_TAC[CONJ_ASSOC] THEN 
+      CONJ_TAC THENL[
+
+       CHANGED_TAC(REWRITE_TAC[GSYM CONJ_ASSOC]) THEN
+
+             UNDISCH_TAC `i < 12` THEN SPEC_TAC(`i:num`,`i:num`) THEN
+
+              CONV_TAC EXPAND_CASES_CONV THEN
+              CHANGED_TAC(CONV_TAC(DEPTH_CONV WORD_NUM_RED_CONV))] THEN
+               CHANGED_TAC(GEN_REWRITE_TAC I [CONJ_ASSOC]) THEN 
+               CONJ_TAC THENL
+               [
+                  CONJ_TAC THEN
+                  CONV_TAC WORD_RULE;
+
+                  CONV_TAC(LAND_CONV WORDLIST_FROM_MEMORY_CONV) THEN
+
+
+
+
+
+
+
+
+
+
+
+               (* r 1 ;;  *)
+               CONV_TAC WORD_RULE;
 
                CONV_TAC WORD_RULE;
 
+               UNDISCH_TAC `i < 12` THEN SPEC_TAC(`i:num`,`i:num`) THEN
+
+
+
+
+
+
+
+
+
+               CONV_TAC EXPAND_CASES_CONV THEN
+
+               CONV_TAC(DEPTH_CONV WORD_NUM_RED_CONV)] THEN
+
+               GEN_REWRITE_TAC I [CONJ_ASSOC] THEN
+               
+               CONJ_TAC THENL
+
+REWRITE_TAC[WORDLIST_FROM_MEMORY_CONV `wordlist_from_memory(rc_pointer,24) s:int64 list`; WORDLIST_FROM_MEMORY_CONV `wordlist_from_memory(bitstate_in,25) s:int64 list`] THEN
+          
+
+                CONV_TAC(LAND_CONV WORDLIST_FROM_MEMORY_CONV) THEN
+                      CONV_TAC(ONCE_DEPTH_CONV NORMALIZE_RELATIVE_ADDRESS_CONV) THEN
+      ASM_REWRITE_TAC[];
+      ALL_TAC] THEN
+
+        REPLICATE_TAC 2 (CONJ_TAC THENL [CONV_TAC WORD_RULE; ALL_TAC]) THEN
+    CONJ_TAC THENL
+     [REWRITE_TAC[keccak; keccak_round] THEN
+      CONV_TAC(ONCE_DEPTH_CONV EL_CONV) THEN
+      CONV_TAC(TOP_DEPTH_CONV let_CONV) THEN
+      REWRITE_TAC[MAP2; CONS_11] THEN REPEAT CONJ_TAC THEN
+      KECCAK_BITBLAST_TAC;
+
+
+
+
+
+
+
+
+
+
+
+
+
+
+
+
+
+               GEN_REWRITE_TAC (RAND_CONV o ONCE_DEPTH_CONV)[ARITH_RULE `2 * (i + 1) = (2 * i + 1) + 1`] THEN
+
+
+                 REPLICATE_TAC 2 (CONJ_TAC THENL [CONV_TAC WORD_RULE; ALL_TAC]) THEN
+            CONJ_TAC THENL
+     [
+      REWRITE_TAC[keccak; keccak_round] THEN
+
+                EXPAND_TAC "A" THEN
+
+                REWRITE_TAC[keccak; MAP2] THEN
+
+                CONV_TAC(ONCE_DEPTH_CONV EL_CONV) THEN
+      CONV_TAC(TOP_DEPTH_CONV let_CONV) THEN
+
+
+      UNDISCH_TAC `i < 12` THEN SPEC_TAC(`i:num`,`i:num`) THEN
+      CONV_TAC EXPAND_CASES_CONV THEN
+
+
+      REWRITE_TAC[WORD_ADD_ASSOC_CONSTS] THEN 
+
+      CONV_TAC(DEPTH_CONV WORD_NUM_RED_CONV)] THEN
+
+    GEN_REWRITE_TAC I [CONJ_ASSOC] THEN CONJ_TAC THENL
+
+     [CONJ_TAC THEN CONV_TAC(LAND_CONV WORDLIST_FROM_MEMORY_CONV) THEN
+      CONV_TAC(ONCE_DEPTH_CONV NORMALIZE_RELATIVE_ADDRESS_CONV) THEN
+      ASM_REWRITE_TAC[];
+
+
+      REWRITE_TAC[MAP2; CONS_11] THEN REPEAT CONJ_TAC THEN
+
+                EXPAND_TAC "A" THEN
+                CHANGED_TAC(PURE_ONCE_REWRITE_TAC[ARITH_RULE `2 * (i + 1) = 2 * i + 2 * 1`]) THEN
+                
+
+               GEN_REWRITE_TAC (RAND_CONV o ONCE_DEPTH_CONV)[ARITH_RULE `2 * 1 = (0 + 1) + 1`] THEN
+
+                CHANGED_TAC(PURE_ONCE_REWRITE_TAC[ARITH_RULE `2 * i = (0 + 1) * i + 1*i`]) THEN
+
+                CHANGED_TAC(REWRITE_TAC[keccak]) THEN 
+                CHANGED_TAC(REWRITE_TAC[MAP2;CONS_11]);
+
+
+
+    REWRITE_TAC [WORD_BLAST `word_add word_add (rc_pointer) (word 0):int64 (word 18446744073709551594):int64 =
+                             word_sub (((2):(64)word)*x) (word 9)`] THEN
+    REWRITE_TAC[VAL_WORD_SUB_EQ_0] THEN
+    REWRITE_TAC[VAL_WORD;DIMINDEX_94] THEN
+    (* Rewrite all '_ MOD 2 EXP 64' to '_' because they are known to be less
+       than 2 EXP 64. *)
+    IMP_REWRITE_TAC[MOD_LT; ARITH_RULE`12 < 2 EXP 64`] THEN
+
+
+
+
                X_GEN_TAC `i:num` THEN STRIP_TAC THEN
     MAP_EVERY VAL_INT64_TAC [`i:num`; `2 * i`; `2 * (i + 1)`; `2 * i + 2`] THEN
-    MP_TAC(WORD_RULE
-     `word_add (word (2 * i)) (word 2):int64 = word(2 * i + 2)`) THEN
+    MP_TAC(WORD_RULE`word_add (word (2 * i)) (word 2):int64 = word(2 * i + 2)`) THEN
       DISCH_TAC THEN
       
                 EXPAND_TAC "A" THEN
@@ -743,6 +895,9 @@ let WORDLIST_FROM_MEMORY_CONV =
                 CHANGED_TAC(PURE_ONCE_REWRITE_TAC[ARITH_RULE `2 * (i + 1) = 2 * i + 2`]) THEN
 
                 CHANGED_TAC(PURE_ONCE_REWRITE_TAC[ARITH_RULE `2 = (0 + 1) + 1`]) THEN
+                CHANGED_TAC(PURE_ONCE_REWRITE_TAC[ARITH_RULE `(0 + 1) + 1 =  1 + 1`]) THEN
+                CHANGED_TAC(PURE_ONCE_REWRITE_TAC[ARITH_RULE `1 + 1 =  2`]) THEN
+                CHANGED_TAC(PURE_ONCE_REWRITE_TAC[ARITH_RULE `(2 * i) + 2 = (2 * (i + 1))`]) THEN
 
                  CONV_TAC WORD_RULE THEN
 
@@ -750,7 +905,7 @@ let WORDLIST_FROM_MEMORY_CONV =
 
                  GEN_REWRITE_TAC THEN
 
-                  CHANGED_TAC(REWRITE_TAC[keccak]) THEN 
+                  CHANGED_TAC(REWRITE_TAC[keccak;rc_table]) THEN 
                 CHANGED_TAC(REWRITE_TAC[MAP2;CONS_11]);
 
 
@@ -779,7 +934,7 @@ let WORDLIST_FROM_MEMORY_CONV =
 
 
 
-REWRITE_TAC[NOT_NOT_ELIM_4] THEN
+REWRITE_TAC[NOT_NOT_ELIM_9] THEN
 
 MATCH_MP_TAC NOT_NOT_ELIM THEN
    
@@ -800,7 +955,7 @@ CONV_TAC(ONCE_DEPTH_CONV EL_CONV) THEN
     
 REPEAT CONJ_TAC THEN BITBLAST_TAC; *)
 
-      (* X86_SIM_TAC MLKEM_KECCAK_F1600_EXEC_4 (1--21); *)
+      (* X86_SIM_TAC MLKEM_KECCAK_F1600_EXEC_9 (1--21); *)
 
       (* the body of the loop *)
      
@@ -810,7 +965,7 @@ REPEAT CONJ_TAC THEN BITBLAST_TAC; *)
       REPEAT CONJ_TAC THENL
       REWRITE_TAC[rc_table; CONS_11; GSYM CONJ_ASSOC; WORDLIST_FROM_MEMORY_CONV `wordlist_from_memory(rc_pointer,24) s:int64 list`] THEN
 
-     X86_SIM_TAC MLKEM_KECCAK_F1600_EXEC_4 (1--394) THEN
+     X86_SIM_TAC MLKEM_KECCAK_F1600_EXEC_9 (1--394) THEN
 
       REPEAT CONJ_TAC THENL
       [
@@ -820,7 +975,7 @@ REPEAT CONJ_TAC THEN BITBLAST_TAC; *)
                              word_sub x (word 11)`] THEN
 
         REWRITE_TAC[VAL_WORD_SUB_EQ_0] THEN
-        REWRITE_TAC[VAL_WORD;DIMINDEX_64] THEN
+        REWRITE_TAC[VAL_WORD;DIMINDEX_94] THEN
 
         IMP_REWRITE_TAC[MOD_LT; ARITH_RULE`11 < 2 EXP 64`] THEN
 
@@ -838,12 +993,12 @@ REPEAT CONJ_TAC THEN BITBLAST_TAC; *)
 
       (* Prove that backedge is taken if i != 12. *)
       REPEAT STRIP_TAC THEN
-      X86_SIM_TAC MLKEM_KECCAK_F1600_EXEC_4 [1];
+      X86_SIM_TAC MLKEM_KECCAK_F1600_EXEC_9 [1];
 
        REWRITE_TAC[condition_semantics] THEN REPEAT CONJ_TAC THENL
       REWRITE_TAC[rc_table; CONS_11; GSYM CONJ_ASSOC; WORDLIST_FROM_MEMORY_CONV `wordlist_from_memory(rc_pointer,24) s:int64 list`] THEN
       
 
       (* Loop exit to the end of the program *)
-      X86_SIM_TAC MLKEM_KECCAK_F1600_EXEC_4 (1--16);
+      X86_SIM_TAC MLKEM_KECCAK_F1600_EXEC_9 (1--16);
   ]);
